Updates.

HandbookOfPracticalLogicLean/Chapter2/Unification.lean
@@ -316,52 +316,85 @@ example
 -------------------------------------------------------------------------------
 
 
-def decidable_is_small_step
-  (E : List (String × Formula_))
-  (X Y : String) :
-  Prop :=
-  match E with
-  | [] => False
-  | hd :: tl => (hd.fst = X ∧ atom_occurs_in Y hd.snd) ∨
-    decidable_is_small_step tl X Y
-
-
-instance
-  (E : List (String × Formula_))
-  (X Y : String) :
-  Decidable (decidable_is_small_step E X Y) :=
-  by
-  induction E
-  all_goals
-    unfold decidable_is_small_step
-    infer_instance
-
-
-def is_small_step
+def is_small_step_v1
   (E : List (String × Formula_))
   (X Y : String) :
   Prop :=
   ∃ (F : Formula_), (X, F) ∈ E ∧ atom_occurs_in Y F
 
 
-example
+def is_small_step_v2
+  (E : List (String × Formula_))
+  (X Y : String) :
+  Prop :=
+  match E with
+  | [] => False
+  | hd :: tl => (hd.fst = X ∧ atom_occurs_in Y hd.snd) ∨
+    is_small_step_v2 tl X Y
+
+
+instance
+  (E : List (String × Formula_))
+  (X Y : String) :
+  Decidable (is_small_step_v2 E X Y) :=
+  by
+  induction E
+  all_goals
+    unfold is_small_step_v2
+    infer_instance
+
+
+lemma is_small_step_v1_imp_is_small_step_v2
   (E : List (String × Formula_))
   (X Y : String)
-  (h1 : decidable_is_small_step E X Y) :
-  is_small_step E X Y :=
+  (h1 : is_small_step_v1 E X Y) :
+  is_small_step_v2 E X Y :=
   by
   induction E
   case nil =>
-    unfold decidable_is_small_step at h1
+    unfold is_small_step_v1 at h1
+    simp only [List.not_mem_nil] at h1
+    obtain ⟨F, h1_left, h1_right⟩ := h1
     contradiction
   case cons hd tl ih =>
-    unfold decidable_is_small_step at h1
+    unfold is_small_step_v1 at h1
+    obtain ⟨F, h1_left, h1_right⟩ := h1
+    simp only [List.mem_cons] at h1_left
+
+    cases h1_left
+    case inl h1_left =>
+      rewrite [← h1_left]
+      unfold is_small_step_v2
+      simp only
+      left
+      exact ⟨trivial, h1_right⟩
+    case inr h1_left =>
+      unfold is_small_step_v2
+      right
+      apply ih
+      unfold is_small_step_v1
+      apply Exists.intro F
+      exact ⟨h1_left, h1_right⟩
+
+
+lemma is_small_step_v2_imp_is_small_step_v1
+  (E : List (String × Formula_))
+  (X Y : String)
+  (h1 : is_small_step_v2 E X Y) :
+  is_small_step_v1 E X Y :=
+  by
+  induction E
+  case nil =>
+    unfold is_small_step_v2 at h1
+    contradiction
+  case cons hd tl ih =>
+    unfold is_small_step_v2 at h1
 
     cases h1
     case inl h1 =>
       obtain ⟨h1_left, h1_right⟩ := h1
 
-      unfold is_small_step
+      unfold is_small_step_v1
       apply Exists.intro hd.2
       rewrite [← h1_left]
       simp only [List.mem_cons]
@@ -371,10 +404,10 @@ example
       · exact h1_right
     case inr h1 =>
       specialize ih h1
-      unfold is_small_step at ih
+      unfold is_small_step_v1 at ih
       obtain ⟨F, ih_left, ih_right⟩ := ih
 
-      unfold is_small_step
+      unfold is_small_step_v1
       apply Exists.intro F
       constructor
       · simp only [List.mem_cons]
@@ -383,37 +416,14 @@ example
       · exact ih_right
 
 
-example
+lemma is_small_step_v1_iff_is_small_step_v2
   (E : List (String × Formula_))
-  (X Y : String)
-  (h1 : is_small_step E X Y) :
-  decidable_is_small_step E X Y :=
+  (X Y : String) :
+  is_small_step_v1 E X Y ↔ is_small_step_v2 E X Y :=
   by
-  induction E
-  case nil =>
-    unfold is_small_step at h1
-    simp only [List.not_mem_nil] at h1
-    obtain ⟨F, h1_left, h1_right⟩ := h1
-    contradiction
-  case cons hd tl ih =>
-    unfold is_small_step at h1
-    obtain ⟨F, h1_left, h1_right⟩ := h1
-    simp only [List.mem_cons] at h1_left
-
-    cases h1_left
-    case inl h1_left =>
-      rewrite [← h1_left]
-      unfold decidable_is_small_step
-      simp only
-      left
-      exact ⟨trivial, h1_right⟩
-    case inr h1_left =>
-      unfold decidable_is_small_step
-      right
-      apply ih
-      unfold is_small_step
-      apply Exists.intro F
-      exact ⟨h1_left, h1_right⟩
+  constructor
+  · apply is_small_step_v1_imp_is_small_step_v2
+  · apply is_small_step_v2_imp_is_small_step_v1
 
 
 -------------------------------------------------------------------------------
